src/FMap.v
@@ -2636,6 +2636,17 @@ Ltac mred_unit :=
 
 Ltac mred := repeat mred_unit.
 
+Ltac mred_find :=
+  repeat
+    (match goal with
+     | [H: Some _ = M.find _ _ |- _] => apply eq_sym in H
+     | [H: None = M.find _ _ |- _] => apply eq_sym in H
+     | [H1: M.find ?m ?k1 = Some _, H2: M.find ?m ?k2 = Some _ |- _] =>
+       rewrite H1 in H2; inv H2
+     | [H1: M.find ?m ?k1 = Some _, H2: M.find ?m ?k2 = None |- _] =>
+       rewrite H1 in H2; discriminate
+     end; simpl in *).
+
 Ltac mcontra :=
   repeat
     match goal with
